ρ -> σ
It's more of a state than an environment

Imp/Expr/Eval.lean
@@ -13,12 +13,12 @@ def Env := String → Value
 namespace Env
 
 /-- Set a value in an environment -/
-def set (x : String) (v : Value) (ρ : Env) : Env :=
-  fun y => if x == y then v else ρ y
+def set (x : String) (v : Value) (σ : Env) : Env :=
+  fun y => if x == y then v else σ y
 
 /-- Look up a value in an environment -/
-def get (x : String) (ρ : Env) : Value :=
-  ρ x
+def get (x : String) (σ : Env) : Value :=
+  σ x
 
 /-- Initialize an environment, setting all uninitialized memory to `i` -/
 def init (i : Value) : Env := fun _ => i
@@ -27,11 +27,11 @@ def init (i : Value) : Env := fun _ => i
 theorem get_init : (Env.init v).get x = v := by rfl
 
 @[simp]
-theorem get_set_same {ρ : Env} : (ρ.set x v).get x = v := by
+theorem get_set_same {σ : Env} : (σ.set x v).get x = v := by
   simp [get, set]
 
 @[simp]
-theorem get_set_different {ρ : Env} : x ≠ y → (ρ.set x v).get y = ρ.get y := by
+theorem get_set_different {σ : Env} : x ≠ y → (σ.set x v).get y = σ.get y := by
   intros
   simp [get, set, *]
 
@@ -65,13 +65,13 @@ Evaluates an expression, finding the value if it has one.
 
 Expressions that divide by zero don't have values - the result is undefined.
 -/
-def eval (ρ : Env) : Expr → Option Value
+def eval (σ : Env) : Expr → Option Value
   | .const i => some i
-  | .var x => ρ.get x
+  | .var x => σ.get x
   | .un op e => do
-    let v ← e.eval ρ
+    let v ← e.eval σ
     op.apply v
   | .bin op e1 e2 => do
-    let v1 ← e1.eval ρ
-    let v2 ← e2.eval ρ
+    let v1 ← e1.eval σ
+    let v2 ← e2.eval σ
     op.apply v1 v2
